To prove $\widehat{v}^3 = -\widehat{v}$, where $\widehat{v} \in \mathbb{R}^{3 \times 3}$ is the skew-symmetric matrix corresponding to the vector $v \in \mathbb{R}^3$ with $||v|| = 1$ such that the cross product $v \times x = \widehat{v} x$ for all $x \in \mathbb{R}^3$, we use the given hint $\widehat{v}^2 = v v^T - I$.

Since $\widehat{v}$ is skew-symmetric, $\widehat{v}^T = -\widehat{v}$. Now, compute $\widehat{v}^3 = \widehat{v} \cdot \widehat{v}^2 = \widehat{v} (v v^T - I)$.

First, consider $\widehat{v} (v v^T)$:
- $v v^T$ is a rank-1 matrix, and $\widehat{v} v = 0$ because the cross product of a vector with itself is zero.
- Thus, $\widehat{v} (v v^T) = 0$.

Next, consider $\widehat{v} (-I) = -\widehat{v}$.

So, $\widehat{v}^3 = \widehat{v} (v v^T - I) = 0 - \widehat{v} = -\widehat{v}$.

Hence, $\widehat{v}^3 = -\widehat{v}$.

---

### Is the condition $||v||=1$ redundant?

The condition $||v||=1$ is **not** redundant. It is essential for the proof.

The hint provided, $\widehat{v}^2 = v v^T - I$, is a specific case of the more general vector triple product rule in matrix form, which is:
$$ \widehat{v}^2 = v v^T - ||v||^2 I $$

This general formula is valid for any vector $v \in \mathbb{R}^3$. The hint in the problem statement implicitly uses the condition $||v||=1$ to simplify the general formula.

Let's see what happens if we use the general formula to compute $\widehat{v}^3$:
$$ \widehat{v}^3 = \widehat{v} \cdot \widehat{v}^2 = \widehat{v} (v v^T - ||v||^2 I) $$
$$ \widehat{v}^3 = \widehat{v}(v v^T) - \widehat{v}(||v||^2 I) $$

As shown in the original proof, the term $\widehat{v}(v v^T)$ is equal to the zero matrix. This leaves us with:
$$ \widehat{v}^3 = -||v||^2 \widehat{v} $$

For the statement $\widehat{v}^3 = -\widehat{v}$ to be true, we must have:
$$ -||v||^2 \widehat{v} = -\widehat{v} $$

This equation only holds if $\widehat{v}$ is the zero matrix (i.e., $v=0$) or if $||v||^2 = 1$. Since the problem deals with a non-zero vector, the condition $||v||=1$ is necessary.
